working with dune

extracted/test_base64.ml
@@ -1,15 +1,28 @@
 open Base64
 
-let test_val = "Hello, World!"
-
 let string_to_char_list (s: string) : char list =
   List.init (String.length s) (String.get s)
 
 let char_list_to_string (cl: char list) : string =
   String.init (List.length cl) (List.nth cl)
 
-let test_val_list = string_to_char_list test_val
+let usage () =
+  print_endline "Usage: test_base64 [encode|decode] <string>"
 
-let test_enc = standardPaddedStringEncoder.strict_encode test_val_list
-
-let _ = print_endline (char_list_to_string (projT1 test_enc))
+let () = 
+  let args = Array.to_list Sys.argv in
+  let { strict_encode; strict_decode } = standardPaddedStringEncoder in
+  match args with
+  | [ _; "encode"; x ] -> 
+      string_to_char_list x
+      |> strict_encode
+      |> projT1
+      |> char_list_to_string
+      |> print_endline
+  | [ _; "decode"; x ] -> 
+      let __ = let rec f _ = Obj.repr f in Obj.repr f in
+      string_to_char_list x
+      |> fun cl -> strict_decode (ExistT (cl, __))
+      |> char_list_to_string
+      |> print_endline
+  | _ -> usage ()
